CoqOfRust/revm/revm_context_interface/links/journaled_state.v
@@ -1,6 +1,84 @@
 Require Import CoqOfRust.CoqOfRust.
 Require Import CoqOfRust.links.M.
-Require Import CoqOfRust.revm.revm_context_interface.journaled_state.
+Require Import core.links.option.
+Require Import revm.revm_context_interface.journaled_state.
+
+(*
+pub struct StateLoad<T> {
+    pub data: T,
+    pub is_cold: bool,
+}
+*)
+Module StateLoad.
+  Record t {T : Set} : Set := {
+    data : T;
+    is_cold : bool;
+  }.
+  Arguments t : clear implicits.
+
+  Global Instance IsLink {T : Set} `{Link T} : Link (t T) := {
+    Φ := Ty.apply (Ty.path "revm_context_interface::journaled_state::StateLoad") [] [Φ T];
+    φ x :=
+      Value.StructRecord "revm_context_interface::journaled_state::StateLoad" [
+        ("data", φ x.(data));
+        ("is_cold", φ x.(is_cold))
+      ];
+  }.
+
+  Definition of_ty (T_ty : Ty.t) :
+    OfTy.t T_ty ->
+    OfTy.t (Ty.apply (Ty.path "revm_context_interface::journaled_state::StateLoad") [] [T_ty]).
+  Proof.
+    intros [T].
+    eapply OfTy.Make with (A := t T).
+    now subst.
+  Defined.
+  Smpl Add apply of_ty : of_ty.
+
+  Lemma of_value_with (T : Set) `{Link T}
+      (data : T) data'
+      (is_cold : bool) is_cold' :
+    data' = φ data ->
+    is_cold' = φ is_cold ->
+    Value.StructRecord "revm_context_interface::journaled_state::StateLoad" [
+      ("data", data');
+      ("is_cold", is_cold')
+    ] = φ (Build_t _ data is_cold).
+  Proof.
+    now intros; subst.
+  Qed.
+  Smpl Add eapply of_value_with : of_value.
+
+  Module SubPointer.
+    Definition get_data (T : Set) `{Link T} : SubPointer.Runner.t (t T)
+      (Pointer.Index.StructRecord "revm_context_interface::journaled_state::StateLoad" "data") :=
+    {|
+      SubPointer.Runner.projection x := Some x.(data);
+      SubPointer.Runner.injection x y := Some (x <| data := y |>);
+    |}.
+
+    Lemma get_data_is_valid (T : Set) `{Link T} :
+      SubPointer.Runner.Valid.t (get_data T).
+    Proof.
+      now constructor.
+    Qed.
+    Smpl Add apply get_data_is_valid : run_sub_pointer.
+
+    Definition get_is_cold (T : Set) `{Link T} : SubPointer.Runner.t (t T)
+      (Pointer.Index.StructRecord "revm_context_interface::journaled_state::StateLoad" "is_cold") :=
+    {|
+      SubPointer.Runner.projection x := Some x.(is_cold);
+      SubPointer.Runner.injection x y := Some (x <| is_cold := y |>);
+    |}.
+
+    Lemma get_is_cold_is_valid (T : Set) `{Link T} :
+      SubPointer.Runner.Valid.t (get_is_cold T).
+    Proof.
+      now constructor.
+    Qed.
+    Smpl Add apply get_is_cold_is_valid : run_sub_pointer.
+  End SubPointer.
+End StateLoad.
 
 (*
 pub struct Eip7702CodeLoad<T> {
@@ -9,11 +87,90 @@ pub struct Eip7702CodeLoad<T> {
 }
 *)
 Module Eip7702CodeLoad.
-  Parameter t : forall (T : Set), Set.
+  Record t {T : Set} : Set := {
+    state_load : StateLoad.t T;
+    is_delegate_account_cold : option bool;
+  }.
+  Arguments t : clear implicits.
 
-  Global Instance IsLink {T : Set} `{Link T} : Link (t T).
-  Admitted.
+  Global Instance IsLink {T : Set} `{Link T} : Link (t T) :=
+  {
+    Φ := Ty.apply (Ty.path "revm_context_interface::journaled_state::Eip7702CodeLoad") [] [Φ T];
+    φ x :=
+      Value.StructRecord "revm_context_interface::journaled_state::Eip7702CodeLoad" [
+        ("state_load", φ x.(state_load));
+        ("is_delegate_account_cold", φ x.(is_delegate_account_cold))
+      ];
+  }.
+
+  Definition of_ty (T_ty : Ty.t) :
+    OfTy.t T_ty ->
+    OfTy.t (Ty.apply (Ty.path "revm_context_interface::journaled_state::Eip7702CodeLoad") [] [T_ty]).
+  Proof.
+    intros [T].
+    eapply OfTy.Make with (A := t T).
+    now subst.
+  Defined.
+  Smpl Add apply of_ty : of_ty.
+
+  Lemma of_value_with state_load state_load' is_delegate_account_cold is_delegate_account_cold' :
+    state_load' = φ state_load ->
+    is_delegate_account_cold' = φ is_delegate_account_cold ->
+    Value.StructRecord "revm_context_interface::journaled_state::Eip7702CodeLoad" [
+      ("state_load", state_load');
+      ("is_delegate_account_cold", is_delegate_account_cold')
+    ] = φ (Build_t _ state_load is_delegate_account_cold).
+  Proof.
+    now intros; subst.
+  Qed.
+  Smpl Add apply of_value_with : of_value.
+
+  Module SubPointer.
+    Definition get_state_load (T : Set) `{Link T} : SubPointer.Runner.t (t T)
+      (Pointer.Index.StructRecord "revm_context_interface::journaled_state::Eip7702CodeLoad" "state_load") :=
+    {|
+      SubPointer.Runner.projection x := Some x.(state_load);
+      SubPointer.Runner.injection x y := Some (x <| state_load := y |>);
+    |}.
+
+    Lemma get_state_load_is_valid (T : Set) `{Link T} :
+      SubPointer.Runner.Valid.t (get_state_load T).
+    Proof.
+      now constructor.
+    Qed.
+    Smpl Add apply get_state_load_is_valid : run_sub_pointer.
+
+    Definition get_is_delegate_account_cold (T : Set) `{Link T} : SubPointer.Runner.t (t T)
+      (Pointer.Index.StructRecord "revm_context_interface::journaled_state::Eip7702CodeLoad" "is_delegate_account_cold") :=
+    {|
+      SubPointer.Runner.projection x := Some x.(is_delegate_account_cold);
+      SubPointer.Runner.injection x y := Some (x <| is_delegate_account_cold := y |>);
+    |}.
+
+    Lemma get_is_delegate_account_cold_is_valid (T : Set) `{Link T} :
+      SubPointer.Runner.Valid.t (get_is_delegate_account_cold T).
+    Proof.
+      now constructor.
+    Qed.
+    Smpl Add apply get_is_delegate_account_cold_is_valid : run_sub_pointer.
+  End SubPointer.
 End Eip7702CodeLoad.
+
+Module Impl_Eip7702CodeLoad.
+  Definition Self (T : Set) `{Link T} : Set :=
+    Eip7702CodeLoad.t T.
+
+  (* pub fn into_components(self) -> (T, Eip7702CodeLoad<()>) *)
+  Instance run_into_components (T : Set) `{Link T} (self : Self T) :
+    Run.Trait
+      (journaled_state.Impl_revm_context_interface_journaled_state_Eip7702CodeLoad_T.into_components (Φ T))
+      [] [] [ φ self ] (T * Self unit).
+  Proof.
+    constructor.
+    run_symbolic.
+  Admitted.
+End Impl_Eip7702CodeLoad.
+Export Impl_Eip7702CodeLoad.
 
 (*
 pub struct AccountLoad {
@@ -100,16 +257,3 @@ Module AccountLoad.
     Smpl Add apply get_is_empty_is_valid : run_sub_pointer.
   End SubPointer.
 End AccountLoad.
-
-(*
-pub struct StateLoad<T> {
-    pub data: T,
-    pub is_cold: bool,
-}
-*)
-Module StateLoad.
-  Parameter t : forall (T : Set), Set.
-
-  Global Instance IsLink {T : Set} `{Link T} : Link (t T).
-  Admitted.
-End StateLoad.
