CoqOfRust/revm/revm_interpreter/instructions/links/contract.v
@@ -57,6 +57,7 @@ Proof.
   constructor.
   destruct run_InterpreterTypes_for_WIRE eqn:?.
   destruct run_StackTrait_for_Stack.
+  destruct run_MemoryTrait_for_Memory.
   destruct run_LoopControl_for_Control.
   destruct run_Immediates_for_Bytecode.
   destruct run_Jumps_for_Bytecode.
@@ -68,9 +69,6 @@ Proof.
   destruct links.mod.Impl_Deref_for_Bytes.run.
   destruct (Impl_Into_for_From_T.run Impl_From_Vec_u8_for_Bytes.run).
   run_symbolic.
-  (* "synthetic" values appearing in the translation *)
-  admit.
-  all: fail.
 Admitted.
 
 (*
