CoqOfRust/revm/revm_interpreter/instructions/links/utility.v
@@ -142,3 +142,4 @@ Module Impl_IntoAddress_for_U256.
     IntoAddress.into_address := run_into_address;
   }.
 End Impl_IntoAddress_for_U256.
+Export Impl_IntoAddress_for_U256.
